EbpfVerifierRangeAnalysis/ALU.lean
@@ -1,5 +1,6 @@
 import Std
 import Mathlib.Data.Int.Init
+import Mathlib.Data.Nat.ModEq
 import EbpfVerifierRangeAnalysis.Overflow
 import EbpfVerifierRangeAnalysis.Register
 
@@ -7,15 +8,42 @@ import EbpfVerifierRangeAnalysis.Register
 
 -- **Addition**
 
+
+
+lemma aux {a b a' b' : UInt32} (h : a.toNat + b.toNat < UInt32.size) (h' : a'.toNat + b'.toNat < UInt32.size)
+    (hn : a.toNat + b.toNat ≤ a'.toNat + b'.toNat) :
+    a + b ≤ a' + b' := by
+  change (a + b).toNat ≤ (a' + b').toNat
+  simp only [UInt32.toNat_add]
+  rw [Nat.add_mod_of_add_mod_lt, Nat.add_mod_of_add_mod_lt]
+  · simpa using hn
+  · simpa using h'
+  · simpa using h
+
+
 def scalar_add_32(a b: BpfRegister) : BpfRegister :=
-  let (u32_min, u32_max) := if unsignedCheckAddOverflow32 a.u32_min b.u32_min ∨
+-- pattern matching (have v let)
+  let res := if unsignedCheckAddOverflow32 a.u32_min b.u32_min ∨
     unsignedCheckAddOverflow32 a.u32_max b.u32_max then
     (0, UInt32_max)
     else
     (a.u32_min + b.u32_min, a.u32_max + b.u32_max)
   {
-    u32_min := u32_min,
-    u32_max := u32_max,
+    u32_min := res.1,
+    u32_max := res.2,
+    well_formed := by
+      revert res
+      split_ifs
+      · simp
+      · simp
+        rename_i h
+        simp at h
+        apply aux
+        · simp [UInt32.size]
+          omega
+        · simp [UInt32.size]
+          omega
+        · exact Nat.add_le_add a.well_formed b.well_formed
     var_off    := a.var_off
   }
 
@@ -23,21 +51,24 @@ def scalar_add_32(a b: BpfRegister) : BpfRegister :=
 theorem scalar_add_32_bounds_min (a b : BpfRegister) :
   (scalar_add_32 a b).u32_min ≤  a.u32_min + b.u32_min := by
   unfold scalar_add_32
+  simp
   split_ifs with h
   · simp
   · simp
 
--- TODO: Version 2
 @[simp]
 theorem scalar_add_32_bounds_max (a b : BpfRegister) :
   (scalar_add_32 a b).u32_max ≥  a.u32_max + b.u32_max := by
   unfold scalar_add_32
+  simp
   split_ifs with h
   · simp
     unfold UInt32_max
     simp
     bv_decide
   · simp
+
+
 
 theorem scalar_add_32_bounds ( a b : BpfRegister) :
   ((scalar_add_32 a b).u32_min ≤ a.u32_min + b.u32_min) ∧
@@ -47,13 +78,4 @@ theorem scalar_add_32_bounds ( a b : BpfRegister) :
   split_ands
   · simp -- sum is le added components (modulo) (bounds_min)
   · simp -- sum is ge added components (modulo) (bounds_max)
-  ·      -- max is always ge min
-    unfold scalar_add_32
-    simp
-    split_ifs
-    · simp -- overflow occurs
-    · simp -- this case is strange
-      -- bv_decide
-      sorry -- :(
-
--- **Subtraction**
+  · apply BpfRegister.well_formed     -- max is always ge min
